Rename dcontains to deep_contains

state/TargetLangHS.fst
@@ -15,44 +15,44 @@ type rref (t:Type) = r:(reference t){
 
 (** target_lang is a shallow embedding of STLC **)
 class target_lang (t:Type) = {
-  dcontains : t -> mem -> Type0;
+  deep_contains : mem -> t -> Type0;
   has_frame : t -> rid -> Type0; (** shallow check of the region of a value **)
   regional : t -> mem -> rid -> Type0; (** deep check of the region of a value **)
   deep_recall : (r:t) -> Stack unit 
               (requires (fun h -> True))
-              (ensures  (fun h0 _ h1 -> h0 == h1 /\ r `dcontains` h1))
+              (ensures  (fun h0 _ h1 -> h0 == h1 /\ h1 `deep_contains` r))
 }
 
 instance target_lang_unit : target_lang unit = {
-  dcontains = (fun _ _ -> True);
+  deep_contains = (fun _ _ -> True);
   has_frame = (fun _ _ -> True);
   regional = (fun _ _ _ -> True);
   deep_recall = (fun _ -> ())
 }
 
 instance target_lang_int : target_lang int = {
-  dcontains = (fun _ _ -> True);
+  deep_contains = (fun _ _ -> True);
   has_frame = (fun _ _ -> True);
   regional = (fun _ _ _ -> True);
   deep_recall = (fun _ -> ());
 }
 
 instance target_lang_pair (t1:Type) (t2:Type) {| c1:target_lang t1 |} {| c2:target_lang t2 |} : target_lang (t1 * t2) = {
-  dcontains = (fun (x1, x2) h -> c1.dcontains x1 h /\ c2.dcontains x2 h);
-  has_frame = (fun (x1, x2) rr -> c1.has_frame x1 rr /\ c2.has_frame x2 rr);
+  deep_contains = (fun h (x1, x2) -> h `deep_contains` x1 /\ h `deep_contains` x2);
+  has_frame = (fun (x1, x2) rr -> x1 `has_frame` rr /\ x2 `has_frame` rr);
   regional = (fun (x1, x2) h rr -> c1.regional x1 h rr /\ c2.regional x2 h rr);
   deep_recall = (fun (x1, x2) -> c1.deep_recall x1; c2.deep_recall x2)
 }
 
 instance target_lang_sum (t1:Type) (t2:Type) {| c1:target_lang t1 |} {| c2:target_lang t2 |} : target_lang (either t1 t2) = {
-  dcontains = (fun x h ->
+  deep_contains = (fun h x ->
     match x with
-    | Inl x1 -> c1.dcontains x1 h
-    | Inr x2 -> c2.dcontains x2 h);
+    | Inl x1 -> h `deep_contains` x1
+    | Inr x2 -> h `deep_contains` x2);
   has_frame = (fun x rr ->
     match x with
-    | Inl x1 -> c1.has_frame x1 rr
-    | Inr x2 -> c2.has_frame x2 rr);
+    | Inl x1 -> x1 `has_frame` rr
+    | Inr x2 -> x2 `has_frame` rr);
   regional = (fun x h rr ->
     match x with
     | Inl x1 -> c1.regional x1 h rr
@@ -64,26 +64,22 @@ instance target_lang_sum (t1:Type) (t2:Type) {| c1:target_lang t1 |} {| c2:targe
 }
 
 instance target_lang_ref (t:Type) {| c:target_lang t |} : target_lang (rref t) = {
-  dcontains = (fun (x:rref t) h -> h `contains` x /\ c.dcontains (sel h x) h);
+  deep_contains = (fun h (x:rref t) -> h `contains` x /\ h `deep_contains` (sel h x));
   has_frame = (fun (x:rref t) rr -> frameOf x == rr);
   regional = (fun (x:rref t) h rr -> frameOf x == rr /\ c.regional (sel h x) h rr);  
-  deep_recall = (fun (x:rref t) ->
-    recall x;
-    let v = !x in
-    c.deep_recall v 
-  )
+  deep_recall = (fun (x:rref t) -> recall x; c.deep_recall !x)
 }
 
 let self_contained_region_inv (rr:erid) (h:mem) : Type0 =
   forall a (c:target_lang (rref a)) (r:rref a). h `contains` r /\ frameOf r == rr ==> 
-    c.dcontains r h /\ c.regional r h rr
+    h `c.deep_contains` r /\ c.regional r h rr
 
 unfold let pre_tgt_arrow
   (rrs:erid)
   (#t1:Type) (x:t1) {| tgtx:target_lang t1 |}
   (h0:mem) =
+  h0 `deep_contains` x /\                                                 (* required to instantiate the properties of modifies *)
   regional x h0 rrs /\                                                    (* x is deeply in region rs *)
-  dcontains x h0 /\                                                       (* required to instantiate the properties of modifies *)
   self_contained_region_inv rrs h0 /\
   is_eternal_region rrs                                                   (* required for using ralloc *)
 
@@ -96,8 +92,8 @@ let post_tgt_arrow
 
   self_contained_region_inv rrs h1 /\
 
-  ((tgtr x).regional r h1 rrs) /\                                        (* x is deeply in region rs *)
-  ((tgtr x).dcontains r h1)
+  (h1 `(tgtr x).deep_contains` r) /\
+  ((tgtr x).regional r h1 rrs)                                           (* x is deeply in region rs *)
 (* TODO: what prevents the computation to allocate things in rp?
     If necessary, we can dissable it by adding the following postcondition:
       forall rrp. disjoint rrp rrs ==> equal_heap_dom rrp h0 h1 -- disables allocation in other regions
@@ -120,7 +116,7 @@ instance target_lang_arrow
   (t2:t1 -> Type)
   {| (x:t1 -> target_lang (t2 x)) |}
   : target_lang (mk_tgt_arrow rrs t1 t2) = {
-    dcontains = (fun _ _ -> True);
+    deep_contains = (fun _ _ -> True);
     has_frame = (fun _ _ -> True);
     regional = (fun _ _ _ -> True);
     deep_recall = (fun _ -> ())
@@ -163,24 +159,24 @@ let elab_typ_tgt (t:typ) (rrs:erid): target_lang (elab_typ t rrs)=
 (** ** Examples **) 
 let write' (#t:Type) {| c:target_lang t |} (r:rref t) (v:t) : ST unit
   (requires (fun h0 -> 
-    dcontains r h0 /\ c.dcontains v h0 /\
+    h0 `deep_contains` r /\ h0 `c.deep_contains` v /\
     regional r h0 (frameOf r) /\ c.regional v h0 (frameOf r) /\
     self_contained_region_inv (frameOf r) h0))
   (ensures (fun h0 u h1 -> 
     assign_post r v h0 u h1 /\
-    dcontains r h1 /\
+    h1 `deep_contains` r /\
     regional r h1 (frameOf r) /\
     self_contained_region_inv (frameOf r) h1))
 = 
   let h0 = get () in
   assert (forall a (c:target_lang (rref a)) (r':rref a). h0 `contains` r' /\ frameOf r' == frameOf r ==> 
-    c.dcontains r' h0 /\ c.regional r' h0 (frameOf r));
+    h0 `c.deep_contains` r' /\ c.regional r' h0 (frameOf r));
   r := v;
   let h1 = get () in
-  assume (dcontains r h1);
+  assume (h1 `deep_contains` r);
   assume (regional r h1 (frameOf r));
   assume (forall a (c:target_lang (rref a)) (r':rref a). 
-    h1 `contains` r' /\ frameOf r' == frameOf r ==> c.dcontains r' h1 /\ c.regional r' h1 (frameOf r))
+    h1 `contains` r' /\ frameOf r' == frameOf r ==> h1 `c.deep_contains` r' /\ c.regional r' h1 (frameOf r))
 
 
 val ralloc' (#a:Type) {| c:target_lang a |} (i:erid) (init:a)
@@ -203,7 +199,7 @@ let sep
   (#trs:Type) (rs:trs) {| tgt_rs: target_lang trs |}
   (rrs:erid)
   h =
-  dcontains rp h /\ dcontains rs h /\                       (* required to instantiate the properties of modifies *)                                            (* separation *)
+  h `deep_contains` rp /\ h `deep_contains` rs /\           (* required to instantiate the properties of modifies *)                                            (* separation *)
   disjoint rrp rrs /\                                       (* ensures disjointness of regions *)
   regional rp h rrp /\ regional rs h rrs 
 
@@ -407,11 +403,11 @@ let rec regional_implies_has_frame #rrs #t (x:elab_typ t rrs)
       ()
   end
 
-let rec dcontais_in_self_contained_implies_regional #rrs #t (x:elab_typ t rrs)
+let rec dcontains_in_self_contained_implies_regional #rrs #t (x:elab_typ t rrs)
 : Stack unit
     (requires (fun h0 ->
       (elab_typ_tgt t rrs).has_frame x rrs
-      /\ (elab_typ_tgt t rrs).dcontains x h0
+      /\ (elab_typ_tgt t rrs).deep_contains h0 x
       /\ self_contained_region_inv rrs h0
       ))
     (ensures (fun h0 _ h1 -> h0 == h1 /\
@@ -423,13 +419,13 @@ let rec dcontais_in_self_contained_implies_regional #rrs #t (x:elab_typ t rrs)
   | TSum t1 t2 -> begin
       let x : either (elab_typ t1 rrs) (elab_typ t2 rrs) = x in
       match x with 
-      | Inl x1 -> dcontais_in_self_contained_implies_regional x1
-      | Inr x2 -> dcontais_in_self_contained_implies_regional x2
+      | Inl x1 -> dcontains_in_self_contained_implies_regional x1
+      | Inr x2 -> dcontains_in_self_contained_implies_regional x2
   end
   | TPair t1 t2 -> begin
       let (x1, x2) : (elab_typ t1 rrs * elab_typ t2 rrs) = x in
-      dcontais_in_self_contained_implies_regional x1;
-      dcontais_in_self_contained_implies_regional x2
+      dcontains_in_self_contained_implies_regional x1;
+      dcontains_in_self_contained_implies_regional x2
   end
   | TRef t -> begin
       let x : rref (elab_typ t rrs) = x in
@@ -509,7 +505,7 @@ let rec elab_exp
     let Some tx = g vx in
     let x : elab_typ tx = ve vx in
     (elab_typ_tgt tx).deep_recall x;
-    dcontais_in_self_contained_implies_regional #rrs #tx x;
+    dcontains_in_self_contained_implies_regional #rrs #tx x;
     x
   | TyApp #_ #_ #_ #tx #tres tyj_f tyj_x ->
     assert ((elab_typ t) == (elab_typ tres));
@@ -517,7 +513,7 @@ let rec elab_exp
     regional_implies_has_frame #rrs #tx x;
     let f : elab_typ (TArr tx tres) = elab_exp tyj_f ve in
     (elab_typ_tgt tx).deep_recall x;
-    dcontais_in_self_contained_implies_regional #rrs #tx x;
+    dcontains_in_self_contained_implies_regional #rrs #tx x;
     elab_apply_arrow rrs tx tres f x
 
   | TyInl #_ #_ #t1 #t2 tyj_1 ->
@@ -533,13 +529,13 @@ let rec elab_exp
       regional_implies_has_frame #rrs #tl x;
       let f : elab_typ (TArr tl tres) = elab_exp tyj_l ve in
       (elab_typ_tgt tl).deep_recall x;
-      dcontais_in_self_contained_implies_regional #rrs #tl x;
+      dcontains_in_self_contained_implies_regional #rrs #tl x;
       elab_apply_arrow rrs tl tres f x
     | Inr y ->
       regional_implies_has_frame #rrs #tr y;
       let f : elab_typ (TArr tr tres) = elab_exp tyj_r ve in
       (elab_typ_tgt tr).deep_recall y;
-      dcontais_in_self_contained_implies_regional #rrs #tr y;
+      dcontains_in_self_contained_implies_regional #rrs #tr y;
       elab_apply_arrow rrs tr tres f y
   end
 
@@ -554,6 +550,6 @@ let rec elab_exp
     regional_implies_has_frame #rrs #tf vf;
     let vs : elab_typ ts = elab_exp tyj_s ve in
     (elab_typ_tgt tf).deep_recall vf;
-    dcontais_in_self_contained_implies_regional #rrs #tf vf;
+    dcontains_in_self_contained_implies_regional #rrs #tf vf;
     (vf, vs)
   #pop-options
